Check for functions that always raise an exception
Functions such as AArch64_TakeException raise a Sail exception to signal
an architectural exception.  Collect those functions and use this
information in register footprint calculation to distinguish between the
successful and the exception case.

tools/analyse_sail.ml
@@ -10,9 +10,13 @@ type fun_info =
     effect : effect;
     calls : IdSet.t;
     regs_read : IdSet.t;
+    regs_read_no_exc : IdSet.t;
     regs_written : IdSet.t;
+    regs_written_no_exc : IdSet.t;
     trans_regs_read : IdSet.t;
-    trans_regs_written : IdSet.t }
+    trans_regs_read_no_exc : IdSet.t;
+    trans_regs_written : IdSet.t;
+    trans_regs_written_no_exc : IdSet.t }
 
 let called_funs_in_exp exp =
   (fold_exp
@@ -48,7 +52,45 @@ let regs_written_in_exp exp =
       lEXP_field = (fun (ids, id) -> IdSet.union ids (reg_idset id)) }
     exp
 
-let add_fun_infos_of_def env fun_infos = function
+let exp_fails exception_funs exp =
+  (* First replace assert(false) with a more obviously failing expression
+     so that we can then use pure_exp_alg below *)
+  let is_false_exp = function
+    | E_aux (E_lit (L_aux (L_false, _)), _) -> true
+    | _ -> false
+  in
+  let exp =
+    fold_exp
+      { id_exp_alg with
+        e_assert = (fun (e, msg) -> if is_false_exp e then E_throw e else E_assert (e, msg)) }
+      exp
+  in
+  fold_exp
+    { (pure_exp_alg false (||)) with
+      e_throw = (fun _ -> true);
+      e_exit = (fun _ -> true);
+      e_app = (fun (id, es) -> List.fold_left (||) (IdSet.mem id exception_funs) es);
+      e_app_infix = (fun (e1, id, e2) -> e1 || IdSet.mem id exception_funs || e2);
+      e_if = (fun (c, e1, e2) -> c || (e1 && e2));
+      e_case = (fun (e, cases) -> e || (cases <> [] && List.fold_left (&&) true cases));
+      (* try-catch might or might not fail, but for our analysis non-failure is the conservative answer *)
+      e_try = (fun _ -> false) }
+    exp
+
+let add_exception_fun exception_funs = function
+  | DEF_fundef (FD_aux (FD_function (_, _, _, funcls), _) as fd) ->
+     let id = id_of_fundef fd in
+     let pexp_fails pexp =
+       let (_, guard, exp, _) = destruct_pexp pexp in
+       exp_fails exception_funs exp || (match guard with Some exp -> exp_fails exception_funs exp | _ -> false)
+     in
+     let funcl_fails (FCL_aux (FCL_Funcl (_, p), _)) = pexp_fails p in
+     if List.for_all funcl_fails funcls then IdSet.add id exception_funs else exception_funs
+  | _ -> exception_funs
+
+let exception_funs defs = List.fold_left add_exception_fun IdSet.empty defs
+
+let add_fun_infos_of_def env exception_funs fun_infos = function
   | DEF_fundef (FD_aux (FD_function (_, _, _, funcls), _) as fd) ->
      let id = id_of_fundef fd in
      let exp_of_pexp pexp =
@@ -61,27 +103,50 @@ let add_fun_infos_of_def env fun_infos = function
      let calls = merge (List.map called_funs_in_exp exps) in
      let calls_infos = Bindings.filter (fun id  _ -> IdSet.mem id calls) fun_infos in
      let regs_read = merge (List.map regs_read_in_exp exps) in
+     let regs_read_no_exc = if IdSet.mem id exception_funs then IdSet.empty else regs_read in
      let regs_written = merge (List.map regs_written_in_exp exps) in
+     let regs_written_no_exc = if IdSet.mem id exception_funs then IdSet.empty else regs_written in
      let trans_regs_read =
        List.map (fun (_, info) -> info.trans_regs_read) (Bindings.bindings calls_infos)
        |> List.fold_left IdSet.union regs_read
+     in
+     let trans_regs_read_no_exc =
+       if IdSet.mem id exception_funs then
+         IdSet.empty
+       else
+         List.map (fun (_, info) -> info.trans_regs_read_no_exc) (Bindings.bindings calls_infos)
+         |> List.fold_left IdSet.union regs_read
      in
      let trans_regs_written =
        List.map (fun (_, info) -> info.trans_regs_written) (Bindings.bindings calls_infos)
        |> List.fold_left IdSet.union regs_written
      in
+     let trans_regs_written_no_exc =
+       if IdSet.mem id exception_funs then
+         IdSet.empty
+       else
+         List.map (fun (_, info) -> info.trans_regs_written_no_exc) (Bindings.bindings calls_infos)
+         |> List.fold_left IdSet.union regs_written
+     in
      let arg_typs, ret_typ, effect = match Type_check.Env.get_val_spec id env with
        | _, Typ_aux (Typ_fn (arg_typs, ret_typ, effect), _) -> arg_typs, ret_typ, effect
        | _ -> raise (Reporting.err_unreachable Parse_ast.Unknown __POS__ ("Function " ^ string_of_id id ^ " does not have function type"))
      in
-     Bindings.add id { arg_typs; ret_typ; effect; calls; regs_read; regs_written; trans_regs_read; trans_regs_written } fun_infos
+     Bindings.add id
+       {
+         arg_typs; ret_typ; effect; calls; regs_read; regs_read_no_exc; regs_written; regs_written_no_exc;
+         trans_regs_read; trans_regs_read_no_exc; trans_regs_written; trans_regs_written_no_exc
+       }
+       fun_infos
   | DEF_internal_mutrec _ ->
      raise (Reporting.err_todo Parse_ast.Unknown "Analysis of mutually recursive functions not implemented")
   | _ -> fun_infos
 
 let fun_ids defs = List.concat (List.map (function DEF_fundef fd -> [id_of_fundef fd] | _ -> []) defs)
 
-let fun_infos_of_defs env defs = List.fold_left (add_fun_infos_of_def env) Bindings.empty defs
+let fun_infos_of_defs env defs =
+  let exc_funs = exception_funs defs in
+  List.fold_left (add_fun_infos_of_def env exc_funs) Bindings.empty defs
 
 let load_files ?mutrecs:(mutrecs=IdSet.empty) files =
   let open Process_file in
